added server-side code for stateless retry in TLS.Cookie; restored some verification in Negotiation

src/tls/Extensions.fst
@@ -1,25 +1,30 @@
 (* Copyright (C) 2012--2017 Microsoft Research and INRIA *)
 module Extensions
 
+(*
 #push-options "--admit_smt_queries true"
 
 let cext_of_custom_aux ((n, e):custom_extension) : clientHelloExtension =
   CHE_Unknown_extensionType n e
 
 let cext_of_custom el =
-  List.Tot.map cext_of_custom_aux el
+  let el = List.Tot.map cext_of_custom_aux el in
+  assume(Parsers.ClientHelloExtensions.clientHelloExtensions_list_bytesize el <= 32000);
+  el
 
 let eext_of_custom_aux ((n, e):custom_extension) =
+  assume(Parsers.EncryptedExtensions.encryptedExtensions_list_bytesize el <= 32000);
   EE_Unknown_extensionType n e
 
 let eext_of_custom el =
-  List.Tot.map eext_of_custom_aux el
+  List.Tot.map eext_of_custom_aux el in
 
 let custom_of_cext_aux = function
   | CHE_Unknown_extensionType n e -> Some (n,e)
   | _ -> None
 
 let custom_of_cext el =
+  // 19-06-17 we miss bytelength-counting maps; we'll get rid of this code anyway.
   List.Tot.choose custom_of_cext_aux el
 
 let custom_of_eext_aux = function
@@ -30,10 +35,12 @@ let custom_of_eext el =
   List.Tot.choose custom_of_eext_aux el
 
 #pop-options
+*)
 
-let clientHelloExtension_of_tagged_unknown_extension (x: taggedUnknownExtension) : Tot clientHelloExtension =
-  match x with
-  | Payload_Unknown_extensionType tg pl -> CHE_Unknown_extensionType tg pl
+let clientHelloExtension_of_tagged_unknown_extension (Payload_Unknown_extensionType tg pl) = 
+  CHE_Unknown_extensionType tg pl
+let encryptedExtension_of_tagged_unknown_extension (Payload_Unknown_extensionType tg pl) = 
+  EE_Unknown_extensionType tg pl
 
 module HS = FStar.HyperStack
 module LP = LowParse.Low
@@ -59,9 +66,15 @@ let valid_clientHelloExtension_of_tagged_unknown_extension
   assert_norm (LP.parse_dsum_kind (LP.get_parser_kind extensionType_repr_parser) clientHelloExtension_sum parse_clientHelloExtension_cases (LP.get_parser_kind clientHelloExtension_CHE_default_parser) == clientHelloExtension_parser_kind);
   LP.valid_dsum_intro_unknown h clientHelloExtension_sum extensionType_repr_parser parse_clientHelloExtension_cases clientHelloExtension_CHE_default_parser sl pos
 
-let clientHelloExtensions_of_tagged_unknown_extensions l = List.Tot.map clientHelloExtension_of_tagged_unknown_extension l
+let clientHelloExtensions_of_unknownExtensions_list l = 
+  List.Tot.map clientHelloExtension_of_tagged_unknown_extension l
 
-#push-options "--z3rlimit 20 --max_fuel 1 --max_ifuel 0"
+let clientHelloExtensions_of_unknownExtensions l = 
+  clientHelloExtensions_of_unknownExtensions_list l
+
+let encryptedExtensions_of_unknownExtensions l = List.Tot.map encryptedExtension_of_tagged_unknown_extension l
+
+#push-options "--z3rlimit 100 --max_fuel 1 --max_ifuel 0"
 let rec valid_list_clientHelloExtensions_of_tagged_unknown_extensions'
   (h: HS.mem)
   (#rrel #rel: _)
@@ -71,7 +84,7 @@ let rec valid_list_clientHelloExtensions_of_tagged_unknown_extensions'
   (requires (LP.valid_list taggedUnknownExtension_parser h sl pos pos'))
   (ensures (
     LP.valid_list clientHelloExtension_parser h sl pos pos' /\
-    LP.contents_list clientHelloExtension_parser h sl pos pos' == clientHelloExtensions_of_tagged_unknown_extensions (LP.contents_list taggedUnknownExtension_parser h sl pos pos')
+    LP.contents_list clientHelloExtension_parser h sl pos pos' == clientHelloExtensions_of_unknownExtensions_list (LP.contents_list taggedUnknownExtension_parser h sl pos pos')
   ))
   (decreases (U32.v pos' - U32.v pos))
 = if pos = pos'
@@ -89,16 +102,9 @@ let rec valid_list_clientHelloExtensions_of_tagged_unknown_extensions'
 
 let valid_list_clientHelloExtensions_of_tagged_unknown_extensions = valid_list_clientHelloExtensions_of_tagged_unknown_extensions'
 
-#push-options "--admit_smt_queries true"
-
-let bindersLen_aux = function
-  | CHE_pre_shared_key psk -> true
-  | _ -> false
 
 let bindersLen che =
-  match List.Tot.find bindersLen_aux che with
+  match List.Tot.find CHE_pre_shared_key? che with
   | None -> 0ul
-  | Some (CHE_pre_shared_key psk) ->
+  | Some (CHE_pre_shared_key psk) -> 
     Parsers.OfferedPsks_binders.offeredPsks_binders_size32 psk.binders
-
-#pop-options
