src/tls/TLS.Cookie.fst
@@ -1,0 +1,122 @@
+module TLS.Cookie
+
+open Mem
+open FStar.Bytes // for the time being
+open TLSConstants
+open TLSError
+
+module CH = Parsers.ClientHello
+
+open Parsers.HRRExtension
+open Parsers.HRRExtensions
+open Parsers.HelloRetryRequest
+
+module Contents = Parsers.MiTLSCookieContents
+
+let prepare_contents (chd:digest) app (hrr: helloRetryRequest) =
+  { Contents.session_id = hrr.session_id;
+    Contents.cipher_suite = hrr.cipher_suite;
+    Contents.group_share = (
+      match find_keyshare hrr with
+      | Some g -> [g]
+      | None -> []);
+    Contents.clientHelloDigest = chd;
+    Contents.extra = app }
+
+
+/// Failures within this code should be prevented by authenticated
+/// encryption, since it covers all contents produced above.
+
+let reconstruct_hrr
+  (raw: encrypted_cookie)
+  (contents: Contents.miTLSCookieContents): result (hrr_leq extensions_max_length)
+=
+  cs <-- (
+    match cipherSuite_of_name contents.Contents.cipher_suite with
+    | Some cs ->
+      if CipherSuite13? cs then
+        Correct cs
+      else
+        fatal Handshake_failure "invalid cookie contents"
+    | _ -> fatal Handshake_failure "invalid cookie contents");
+  let hrr = hrr0 contents.Contents.session_id cs in
+  hrr <-- (
+    match contents.Contents.group_share with
+    | [g] -> correct (append_keyshare hrr g)
+    | []  -> correct #(hrr_leq 16) hrr
+    | _   -> fatal Handshake_failure "invalid cookie contents" );
+  correct #(hrr_leq extensions_max_length) (append_extension 16 hrr (HRRE_cookie raw))
+
+let append chd app hrr =
+  // TODO encrypt
+  let encrypted = Contents.miTLSCookieContents_serializer32 (prepare_contents chd app hrr) in
+  append_extension 16 hrr (HRRE_cookie encrypted)
+
+let decrypt encrypted =
+  // TODO decrypt
+  if length encrypted > encrypted_max_length then
+    fatal Handshake_failure "oversized cookie"
+  else
+  match Contents.miTLSCookieContents_parser32 encrypted with
+  | Some (v,0ul) -> (
+    match reconstruct_hrr encrypted v with
+    | Correct hrr -> correct(v.Contents.clientHelloDigest, v.Contents.extra, hrr)
+    | Error z -> Error z )
+  | _ -> fatal Handshake_failure "invalid cookie contents"
+
+
+
+/// Basic testing---how do I run it?
+
+// Can we get rid of Evercrypt.algs??
+
+let test =
+  let chd = empty_bytes in
+  let hrr = hrr0 empty_bytes (CipherSuite13 EverCrypt.AES128_GCM Spec.Hash.Definitions.SHA2_256) in
+  let extra = empty_bytes in
+  let hrr = append chd extra hrr in
+  match find_cookie hrr with
+  | None -> false
+  | Some c ->
+    match decrypt c with
+    | Error _ -> false
+    | Correct (chd', extra', hrr') ->
+      (chd' = chd && extra' = extra && hrr' = hrr)
+
+
+
+
+// TODO restore debug trace; see below.
+
+(*
+  let hrm = HandshakeMessages.HelloRetryRequest hrr in
+  let hrb = vlbytes 3 (HandshakeMessages.handshakeMessageBytes None hrm) in
+  let plain = hrb @| (vlbytes 1 digest) @| (vlbytes 2 extra) in
+  let cipher = ticket_encrypt false plain in
+  trace ("Encrypting cookie: "^(hex_of_bytes plain));
+  trace ("Encrypted cookie:  "^(hex_of_bytes cipher));
+  cipher
+*)
+
+(*
+  trace ("Decrypting cookie "^(hex_of_bytes b));
+  if length b < 32 then None else
+  match ticket_decrypt false b with
+  | None -> trace ("Cookie decryption failed."); None
+  | Some plain ->
+    trace ("Plain cookie: "^(hex_of_bytes plain));
+    match vlsplit 3 plain with
+    | Error _ -> trace ("Cookie decode error: HRR"); None
+    | Correct (hrb, b) ->
+      let (_, hrb) = split hrb 4ul in // Skip handshake tag and vlbytes 3
+      match HandshakeMessages.parseHelloRetryRequest hrb with
+      | Error (_, m) -> trace ("Cookie decode error: parse HRR, "^m); None
+      | Correct hrr ->
+        match vlsplit 1 b with
+        | Error _ -> trace ("Cookie decode error: digest"); None
+        | Correct (digest, b) ->
+          match vlparse 2 b with
+          | Error _ -> trace ("Cookie decode error: application data"); None
+          | Correct extra ->
+            Some (hrr, digest, extra)
+*)
